extended AMorphism to infinite sets of rules

Term/WithArity/AMorphism.v
@@ -15,6 +15,7 @@ Require Import VecUtil.
 Require Import List.
 Require Import RelUtil.
 Require Import SN.
+Require Import ARules.
 
 Section Morphism.
 
@@ -67,7 +68,9 @@ Qed.
  
 Definition Fr (a : rule S1) := let (l,r) := a in mkRule (Ft l) (Ft r).
 
-Definition Frs := List.map Fr.
+Definition Fl := map Fr.
+
+Definition Frs R a := exists b, R b /\ a = Fr b.
 
 (***********************************************************************)
 (* translation of substitutions in S1 into substitutions in S2 *)
@@ -94,7 +97,7 @@ Lemma Fred : forall R t u, red R t u -> red (Frs R) (Ft t) (Ft u).
 Proof.
 intros. redtac. unfold red. subst.
 exists (Ft l). exists (Ft r). exists (Fc c). exists (Fs s). intuition.
-change (In (Fr (mkRule l r)) (Frs R)). apply in_map. hyp.
+change (Frs R (Fr (mkRule l r))). exists (mkRule l r). intuition.
 rewrite Ft_fill. rewrite Ft_sub. refl.
 rewrite Ft_fill. rewrite Ft_sub. refl.
 Qed.
@@ -104,7 +107,7 @@ Lemma Fhd_red : forall R t u, hd_red R t u -> hd_red (Frs R) (Ft t) (Ft u).
 Proof.
 intros. redtac. unfold hd_red. subst.
 exists (Ft l). exists (Ft r). exists (Fs s). intuition.
-change (In (Fr (mkRule l r)) (Frs R)). apply in_map. hyp.
+change (Frs R (Fr (mkRule l r))). exists (mkRule l r). intuition.
 rewrite Ft_sub. refl. rewrite Ft_sub. refl.
 Qed.
 
@@ -164,6 +167,7 @@ Implicit Arguments Fv [S1 S2 F n].
 Implicit Arguments Fc [S1 S2 F].
 Implicit Arguments Fs [S1 S2 F].
 Implicit Arguments Fr [S1 S2 F].
+Implicit Arguments Fl [S1 S2 F].
 Implicit Arguments Frs [S1 S2 F].
 
 (***********************************************************************)
@@ -174,7 +178,7 @@ Section Preserv.
 Variables S1 S2 : Signature.
 Variables (F : S1 -> S2) (HF : forall f, arity f = arity (F f)).
 Variables (G : S2 -> S1) (HG : forall f, arity f = arity (G f)).
-Variables (E R : rules S1) (E' R' : rules S2).
+Variables (E R : rule S1 -> Prop) (E' R' : rule S2 -> Prop).
 Variables (hyp1 : incl (Frs HG E') E) (hyp2 : incl (Frs HF E) E').
 Variables (hyp3 : incl (Frs HG R') R) (hyp4 : incl (Frs HF R) R').
 
@@ -259,7 +263,7 @@ Proof.
 destruct a as [l r]. simpl. repeat rewrite Ft_epi. refl.
 Qed.
 
-Lemma Frs_epi : forall l, Frs HF (Frs HG l) = l.
+Lemma Fl_epi : forall l, Fl HF (Fl HG l) = l.
 
 Proof.
 induction l; simpl; intros. refl. rewrite Fr_epi. rewrite IHl. refl.
@@ -278,13 +282,21 @@ Variables S1 S2 : Signature.
 Variables (F : S1 -> S2) (HF : forall f, arity f = arity (F f)).
 Variables (G : S2 -> S1) (HG : forall f, arity f = arity (G f)).
 Variables (FG : forall f, F (G f) = f) (GF : forall f, G (F f) = f).
+
+Lemma Frs_incl : forall R, incl (Frs HG (Frs HF R)) R.
+
+Proof.
+intros R x H. do 2 destruct H. subst. do 2 destruct H. subst. rewrite Fr_epi.
+hyp. hyp.
+Qed.
+
 Variables E R : rules S1.
 
 Lemma WF_Fred_iso : WF (red R) <-> WF (red (Frs HF R)).
 
 Proof.
 split; intro. apply WF_Fred with (G:=G) (HG:=HG) (R':=Frs HF R).
-rewrite Frs_epi. apply incl_refl. apply GF. apply incl_refl. hyp.
+apply Frs_incl. apply incl_refl. hyp.
 apply Fred_WF with (S2:=S2) (F:=F) (HF:=HF). hyp.
 Qed.
 
@@ -293,8 +305,7 @@ Lemma WF_Fred_mod_iso : WF (red_mod E R) <-> WF (red_mod (Frs HF E) (Frs HF R)).
 Proof.
 split; intro.
 apply WF_Fred_mod with (G:=G) (HG:=HG) (R':=Frs HF R) (E':=Frs HF E).
-rewrite Frs_epi. apply incl_refl. apply GF. apply incl_refl.
-rewrite Frs_epi. apply incl_refl. apply GF. apply incl_refl. hyp.
+apply Frs_incl. apply incl_refl. apply Frs_incl. apply incl_refl. hyp.
 apply Fred_mod_WF with (S2:=S2) (F:=F) (HF:=HF). hyp.
 Qed.
 
@@ -304,8 +315,7 @@ Lemma WF_Fhd_red_mod_iso :
 Proof.
 split; intro.
 apply WF_Fhd_red_mod with (G:=G) (HG:=HG) (R':=Frs HF R) (E':=Frs HF E).
-rewrite Frs_epi. apply incl_refl. apply GF. apply incl_refl.
-rewrite Frs_epi. apply incl_refl. apply GF. apply incl_refl. hyp.
+apply Frs_incl. apply incl_refl. apply Frs_incl. apply incl_refl. hyp.
 apply Fhd_red_mod_WF with (S2:=S2) (F:=F) (HF:=HF). hyp.
 Qed.
 
